FEC/Verif_field.v
@@ -5,10 +5,9 @@ Require Import CommonVST.
 Require Import Specs.
 Require Import fec.
 Require Import Poly.
+Require Import FECTactics.
 
 Set Bullet Behavior "Strict Subproofs".
-
-Import WPoly.
 
 (** Verification of [fec_find_mod]*)
 (*
@@ -19,15 +18,6 @@ start_function.
 forward_if (PROP () LOCAL (temp _modulus (Vint (Int.repr modulus))) SEP ()).
 *)
 
-(*reflect_iff*)
-
-(*TODO: move to COmmon*)
-Lemma Int_eq_reflect: forall (a b : int),
-  reflect (a = b) (Int.eq a b).
-Proof.
-  intros. destruct (Int.eq a b) eqn : Heq. apply ReflectT. apply Int.same_if_eq; auto.
-  apply ReflectF. apply int_eq_false_e; auto.
-Qed.
 
 (** Verification of [fec_gf_mult] *)
 
@@ -35,13 +25,11 @@ Qed.
 Lemma body_fec_gf_mult : semax_body Vprog Gprog f_fec_gf_mult fec_gf_mult_spec.
 Proof.
   start_function.
-  pose proof fec_n_bound as Fbound.
   forward_if (
     PROP ()
     LOCAL (temp _t'1 (Vint (Int.repr (if Z.eq_dec f 0%Z then 0%Z else if Z.eq_dec g 0%Z then 0%Z else 1%Z)));
      temp _a (Vint (Int.repr f)); temp _b (Vint (Int.repr g)); gvars gv)
-    SEP (data_at Ews (tarray tuchar fec_n) (power_to_index_contents fec_n) (gv _fec_2_index);
-   data_at Ews (tarray tuchar fec_n) index_to_power_contents (gv _fec_2_power))).
+    SEP (INDEX_TABLES gv)).
   - forward. entailer!. f_equal.  
     if_tac. subst. contradiction. if_tac. subst.
     assert (Htriv: Int.eq (Int.repr 0) Int.zero = true).
@@ -52,117 +40,61 @@ Proof.
     apply repr_inj_unsigned in Hz; rep_lia. rewrite Hnon. reflexivity.
   - forward. entailer!. if_tac. reflexivity. 
     apply repr_inj_unsigned in H0; rep_lia.
-  - pose proof modulus_poly_deg_pos as Hpos.
-    pose proof modulus_poly_not_x as Hnotx.
-    pose proof modulus_poly_primitive as Hprim.
-    pose proof modulus_poly_irred as Hirred.
-    pose proof modulus_poly_not_zero as Hnonzero.
-    pose proof modulus_poly_deg_bounds as Hbounds.
-    pose proof modulus_poly_deg as Hdeglog. destruct H.
-    pose proof (polys_deg_bounded _ H) as Hfbound.
-    pose proof (polys_deg_bounded _ H0) as Hgbound.
-    pose proof field_size_fec_n as Hfield_size.
-    forward_if.
-    + destruct H. destruct (Z.eq_dec f 0) as [? | Hf0]. contradiction.
-      destruct (Z.eq_dec g 0) as [? | Hg0]. contradiction.
-      clear H1'. deadvars!.
-      assert (Hfnonzero: poly_of_int f <> zero). { intro Hz. rewrite poly_of_int_zero in Hz. lia. }
-      assert (Hgnonzero: poly_of_int g <> zero). { intro Hz. rewrite poly_of_int_zero in Hz. lia. }
+  - forward_if.
+    + destruct H as [Hf Hg]. destruct (Z.eq_dec f 0) as [? | Hf0]. contradiction.
+      destruct (Z.eq_dec g 0) as [? | Hg0]. contradiction. clear H0 H0'. deadvars!.
+      unfold INDEX_TABLES. Intros.
       forward.
-      * entailer!. rewrite index_to_power_contents_Znth; try lia. simpl.
-        pose proof (find_power_spec mod_poly Hpos Hprim Hnotx (poly_of_int f) Hfnonzero Hfbound) as Hfp.
-        destruct Hfp.
-        pose proof field_size_fec_n. rewrite unsigned_repr; rep_lia.
+      * entailer!. rewrite index_to_power_contents_Znth; try lia. solve_poly_bounds. 
       * forward.
-        -- entailer!. rewrite index_to_power_contents_Znth; try lia. simpl.
-           pose proof (find_power_spec mod_poly Hpos Hprim Hnotx (poly_of_int g) Hgnonzero Hgbound) as Hfp.
-           destruct Hfp.
-           pose proof field_size_fec_n. rewrite unsigned_repr; rep_lia.
-        -- pose proof (find_power_spec mod_poly Hpos Hprim Hnotx (poly_of_int f) Hfnonzero Hfbound) as [Hfp Hfp_bound].
-           pose proof (find_power_spec mod_poly Hpos Hprim Hnotx (poly_of_int g) Hgnonzero Hgbound) as [Hgp Hgp_bound].
-           (*for i + j > fec_n - 1, get conditional in usable form*)
+        -- entailer!. rewrite index_to_power_contents_Znth; try lia. solve_poly_bounds. 
+        -- pose_power (poly_of_int f) Hfp Hfp_bound. pose_power (poly_of_int g) Hgp Hgp_bound.
+          (*for i + j > fec_n - 1, get conditional in usable form*)
            rewrite? index_to_power_contents_Znth; try lia. 
            forward_if.
           ++ forward. (*overflow case*)
-             ** entailer!. rewrite index_to_power_contents_Znth; try lia. simpl.
-                rewrite unsigned_repr; rep_lia.
+             ** entailer!. rewrite index_to_power_contents_Znth; try lia. simpl. solve_poly_bounds.
              ** forward. 
-                --- entailer!. rewrite index_to_power_contents_Znth; try lia. simpl.
-                    rewrite unsigned_repr; rep_lia.
+                --- entailer!. rewrite index_to_power_contents_Znth; try lia. solve_poly_bounds. 
                 --- rewrite !index_to_power_contents_Znth; try lia.
                     forward.
-                  +++ entailer!. rewrite power_to_index_contents_Znth; try lia. simpl.
-                      remember (monomial (Z.to_nat
-                      ((find_power mod_poly (poly_of_int f) + find_power mod_poly (poly_of_int g)) -
-                      (255))) %~ mod_poly) as prod.
-                      pose proof modulus_poly_bound prod as Hprodb. 
-                      assert (Hdeg: deg prod < deg mod_poly) by (rewrite Heqprod; apply pmod_lt_deg; assumption).
-                      specialize (Hprodb Hdeg). rewrite unsigned_repr; rep_lia.
-                  +++ forward. entailer!. (*now, we prove that this actually computes the product for this case*)
-                      rewrite power_to_index_contents_Znth; try lia. f_equal. f_equal. f_equal.
-                      rewrite monomial_add_field_size; try assumption.
-                      replace (Z.to_nat (find_power mod_poly (poly_of_int f) + find_power mod_poly (poly_of_int g) - 
-                      (256 - 1)))
-                      with ((Z.to_nat (find_power mod_poly (poly_of_int f)) +
-                           Z.to_nat (find_power mod_poly (poly_of_int g)) -
-                           Z.to_nat (fec_n - 1))%nat) by (rewrite fec_n_eq; lia).
-                      rewrite <- Hfield_size. replace (Z.to_nat (Z.of_nat (field_size mod_poly))) with
-                      (field_size mod_poly) by lia. 
-                      replace (Z.to_nat (find_power mod_poly (poly_of_int f)) + 
-                        Z.to_nat (find_power mod_poly (poly_of_int g)) - field_size mod_poly + 
-                        field_size mod_poly)%nat with
-                        ((Z.to_nat (find_power mod_poly (poly_of_int f)) + 
-                          Z.to_nat (find_power mod_poly (poly_of_int g)))%nat) by lia.
-                      rewrite <- monomial_exp_law. rewrite pmod_mult_distr; try assumption.
-                      rewrite <- Hfp. rewrite <- Hgp. reflexivity.
+                  +++ entailer!.
+                  +++ entailer!. rewrite power_to_index_contents_Znth; try lia. solve_poly_bounds. rep_lia.
+                  +++ forward. unfold INDEX_TABLES. entailer!. (*now, we prove that this actually computes the product for this case*)
+                      rewrite power_to_index_contents_Znth; try rep_lia. f_equal. f_equal. f_equal.
+                      rewrite Hfp at 2. rewrite Hgp at 2. rewrite <- pmod_mult_distr; [| apply mod_poly_PosPoly].
+                      rewrite (monomial_exp_law). apply (@monomial_powers_eq_mod mod_poly _ mod_poly_PrimPoly).
+                      replace (256 - 1) with (Z.of_nat (field_size mod_poly)) by (rewrite field_size_fec_n; rep_lia).
+                      rewrite Z2Nat.inj_sub by lia. rewrite Z2Nat.inj_add by lia.
+                      rewrite <- (Nat.mod_add _ 1 (field_size mod_poly)). f_equal. rewrite Nat2Z.id. rewrite Nat.mul_1_l.
+                      rewrite Nat.sub_add. reflexivity. all: pose proof field_size_fec_n; rep_lia.
           ++ (*other side of the if statement*) forward.
-            ** entailer!. rewrite index_to_power_contents_Znth; try lia. simpl.
-               rewrite unsigned_repr; rep_lia.
+            ** entailer!. rewrite index_to_power_contents_Znth; try lia. solve_poly_bounds. 
             ** forward. 
-                --- entailer!. rewrite index_to_power_contents_Znth; try lia. simpl.
-                    rewrite unsigned_repr; rep_lia.
-                --- rewrite !index_to_power_contents_Znth; try lia.
-                    assert (Hsumbd: 0 <= find_power mod_poly (poly_of_int f) +
-                       find_power mod_poly (poly_of_int g) < fec_n) by (rewrite fec_n_eq; lia).
-                    forward.
-                  +++ entailer!. rewrite power_to_index_contents_Znth; try lia. remember (monomial (Z.to_nat
-                      ((find_power mod_poly (poly_of_int f) + find_power mod_poly (poly_of_int g)))) %~ mod_poly) 
-                      as prod.
-                      pose proof modulus_poly_bound prod as Hprodb. 
-                      assert (Hdeg: deg prod < deg mod_poly) by (rewrite Heqprod; apply pmod_lt_deg; assumption).
-                      specialize (Hprodb Hdeg). simpl.
-                      rewrite unsigned_repr; rep_lia.
+                --- entailer!. rewrite index_to_power_contents_Znth; try lia. solve_poly_bounds. 
+                --- rewrite !index_to_power_contents_Znth; try lia. forward.
+                  +++ entailer!.
+                  +++ entailer!. rewrite power_to_index_contents_Znth; try lia. solve_poly_bounds. rep_lia. 
                   +++ forward. entailer!. (*now the easier, but similar case*) 
-                      rewrite power_to_index_contents_Znth; try lia. f_equal. f_equal. f_equal. 
-                      replace
-                      (Z.to_nat (find_power mod_poly (poly_of_int f) + find_power mod_poly (poly_of_int g))) with
-                      (Z.to_nat (find_power mod_poly (poly_of_int f)) + 
-                        Z.to_nat (find_power mod_poly (poly_of_int g)))%nat by lia.
-                      rewrite <- monomial_exp_law. rewrite pmod_mult_distr; try assumption.
+                      rewrite power_to_index_contents_Znth; try rep_lia. f_equal. f_equal. f_equal. 
+                      rewrite Z2Nat.inj_add by rep_lia.
+                      rewrite <- monomial_exp_law. rewrite pmod_mult_distr; [| apply mod_poly_PosPoly].
                       rewrite <- Hfp. rewrite <- Hgp. reflexivity.
-    + assert (Hzero: poly_of_int 0%Z = zero). rewrite poly_of_int_zero. lia. if_tac; subst.
-      * forward. entailer!.  rewrite Hzero. rewrite poly_mult_0_l. rewrite pmod_zero; auto.
+    + if_tac; subst.
+      * forward. entailer!. rewrite_zero. rewrite poly_mult_0_l. rewrite pmod_zero; auto. apply mod_poly_PosPoly.
       * if_tac; subst.
-        -- forward. entailer!. rewrite Hzero. rewrite poly_mult_0_r. rewrite pmod_zero; auto.
-        -- inversion H1.
+        -- forward. entailer!. rewrite_zero. rewrite poly_mult_0_r. rewrite pmod_zero; auto. apply mod_poly_PosPoly.
+        -- inversion H0.
 Qed. 
 
 (** Verification of [fec_generate_math_tables]*)
 
-(*TODO: Qed takes a long time (about 70 sec), and I don't know why. It might be unfolding constants or something*)
 Lemma body_fec_generate_math_tables : semax_body Vprog Gprog f_fec_generate_math_tables fec_generate_math_tables_spec.
 Proof.
 start_function.
 forward_call.
-pose proof fec_n_bound as Fbound.
-pose proof modulus_poly_deg_pos as Hpos.
-pose proof modulus_poly_not_x as Hnotx.
-pose proof modulus_poly_primitive as Hprim.
-pose proof modulus_poly_irred as Hirred.
-pose proof modulus_poly_not_zero as Hnonzero.
-pose proof modulus_poly_deg_bounds as Hbounds.
-pose proof modulus_poly_deg as Hdeglog.
-pose proof modulus_pos as Hmodulus.
+pose proof mod_poly_PrimPoly as Hprimpoly.
+pose proof mod_poly_PosPoly as Hpospoly.
 (*loop invariants
   1. fec_2_index: filled out up to ith position, this is relatively straightforward to specity
   2. fec_2_power: is a list l such that for all z, 0 < z < fec_n ->
@@ -181,74 +113,53 @@ pose proof modulus_pos as Hmodulus.
          data_at Ews (tarray tuchar fec_n) (map Vint (map Int.repr (list_repeat (Z.to_nat fec_n) 0%Z)))
      (gv _fec_invefec)))
     break: (PROP () LOCAL (temp _mod (Vint (Int.repr modulus)); gvars gv)
-            SEP (data_at Ews (tarray tuchar fec_n) (power_to_index_contents fec_n) (gv _fec_2_index);
-         data_at Ews (tarray tuchar fec_n) index_to_power_contents (gv _fec_2_power);
+            SEP (INDEX_TABLES gv;
           data_at Ews (tarray tuchar fec_n) (map Vint (map Int.repr (list_repeat (Z.to_nat fec_n) 0%Z)))
      (gv _fec_invefec))).
   - forward. Exists 0%Z. Exists ((list_repeat (Z.to_nat fec_n) 0%Z)). entailer!.
-    rewrite Znth_list_repeat_inrange; lia. simpl. cancel.
+    rewrite Znth_list_repeat_inrange; rep_lia. simpl. cancel.
   - Intros i. Intros l.
     forward_if.
-    + (*Loop body*)  forward_if (PROP (0 <= i <= fec_n /\ 
-      (forall z, 0 < z < fec_n -> 0 < find_power mod_poly (poly_of_int z) < i -> 
-          Znth z l = find_power mod_poly (poly_of_int z)) /\
-      Znth 0 l = 0%Z)
+    + (*Loop body*)  forward_if 
+      (PROP (0 <= i <= fec_n /\ (forall z, 0 < z < fec_n -> 0 < find_power mod_poly (poly_of_int z) < i -> 
+          Znth z l = find_power mod_poly (poly_of_int z)) /\ Znth 0 l = 0%Z)
       LOCAL (temp _mod (Vint (Int.repr modulus)); temp _i (Vint (Int.repr i)); gvars gv)
-      SEP (data_at Ews (tarray tuchar fec_n) (power_to_index_contents (i + 1) ++ map Vint (map Int.repr (list_repeat
-      ((Z.to_nat fec_n) - Z.to_nat (i + 1))%nat 0%Z))) (gv _fec_2_index);
-        data_at Ews (tarray tuchar fec_n) (map Vint (map Int.repr l)) (gv _fec_2_power);
-        data_at Ews (tarray tuchar fec_n) (map Vint (map Int.repr (list_repeat (Z.to_nat fec_n) 0%Z)))
-        (gv _fec_invefec))).
-      * (*i=0 case (base case)*) forward. entailer!.
-        simpl. replace (Z.to_nat fec_n) with (1%nat + (Z.to_nat fec_n - 1))%nat at 1 by lia.
+      SEP (data_at Ews (tarray tuchar fec_n) (power_to_index_contents (i + 1) ++ 
+              map Vint (map Int.repr (list_repeat ((Z.to_nat fec_n) - Z.to_nat (i + 1))%nat 0%Z))) (gv _fec_2_index);
+           data_at Ews (tarray tuchar fec_n) (map Vint (map Int.repr l)) (gv _fec_2_power);
+           data_at Ews (tarray tuchar fec_n) (map Vint (map Int.repr (list_repeat (Z.to_nat fec_n) 0%Z)))
+              (gv _fec_invefec))).
+      * (*i=0 case (base case)*) forward. entailer!. entailer!.
+        simpl. replace (Z.to_nat fec_n) with (1%nat + (Z.to_nat fec_n - 1))%nat at 1 by rep_lia.
         rewrite <- list_repeat_app. simpl. rewrite upd_Znth0. 
         rewrite monomial_0. rewrite pmod_refl; auto. rewrite poly_to_int_one. entailer!.
-        replace (deg one) with (0%Z) by (rewrite deg_one; reflexivity). lia.
-      * (*i <> 0*) assert (Hi1bound: 0 <= poly_to_int (monomial (Z.to_nat (i - 1)) %~ mod_poly) < fec_n). {
-          apply modulus_poly_bound. apply pmod_lt_deg; auto. } 
-        forward. 
+        apply one_lt_deg; auto.
+      * forward. 
         -- (*array access valid*)
-           entailer!. rewrite Znth_app1. 2: list_solve. rewrite power_to_index_contents_Znth. simpl.
-           rewrite unsigned_repr; try rep_lia. lia.
+           entailer!. rewrite Znth_app1. 2: list_solve. rewrite power_to_index_contents_Znth. solve_poly_bounds. lia. 
         -- (*body continue with shift, rewrite shift into polynomial mult*)
            forward. 
-           (*TODO: What is going on here. forward_if takes forever, rewriting doesnt work, the resulting
-              if condition is terrible, even simpl hangs. Is it just because of a constant?*)
+           (*TODO: The resulting if condition is weird for some reason *)
            assert (Hshl : (Int.shl (Int.repr (poly_to_int (monomial (Z.to_nat (i - 1)) %~ mod_poly))) (Int.repr 1)) =
                      (Int.repr (poly_to_int (x *~ (monomial (Z.to_nat (i - 1)) %~ mod_poly))))). {
-           unfold Int.shl. rewrite !unsigned_repr; try rep_lia. rewrite Z.shiftl_mul_pow2; try lia.
-           replace (2 ^ 1) with 2 by lia.
-           assert ((poly_to_int (monomial (Z.to_nat (i - 1)) %~ mod_poly) * 2) = 
-            poly_to_int (x *~ (monomial (Z.to_nat (i - 1)) %~ mod_poly))). {
-            rewrite <- poly_of_int_to_int; try lia. rewrite Z.mul_comm. rewrite poly_shiftl.
-            rewrite poly_of_int_inv. reflexivity. apply modulus_poly_monomial. } f_equal; f_equal; auto. }
-            
-           assert (Hxpoly : (force_val (sem_binary_operation' Oshl tuchar tint (Znth (i - 1)
-                    (power_to_index_contents i ++ map Vint (map Int.repr (list_repeat (Z.to_nat (fec_n - i)) 0%Z))))
-                  (Vint (Int.repr 1)))) = 
-                  (Vint (Int.repr (poly_to_int (x *~ (monomial (Z.to_nat (i - 1)) %~ mod_poly)))))). { 
-           rewrite Znth_app1. 2: rewrite power_to_index_contents_length; lia.
-           rewrite power_to_index_contents_Znth; try lia. simpl. f_equal. apply Hshl. }
-           assert (Hxbound: Int.min_signed <= 
-              poly_to_int (x *~ (monomial (Z.to_nat (i - 1)) %~ mod_poly)) <= Int.max_signed). {
-            (*very annoying proof to prove bounds*)
+           unfold Int.shl. rewrite !unsigned_repr; try rep_lia. 2: solve_poly_bounds. 
+           rewrite Z.shiftl_mul_pow2 by lia. replace (2 ^ 1) with 2 by reflexivity. f_equal.
+           rewrite <- poly_of_int_to_int. 2: pose_poly_bounds; rep_lia. rewrite Z.mul_comm. rewrite poly_shiftl.
+           rewrite poly_of_int_inv. reflexivity. apply modulus_poly_monomial. } rewrite Znth_app1 by solve_prop_length.
+           assert (Hxbound: 0 <= 
+              poly_to_int (x *~ (monomial (Z.to_nat (i - 1)) %~ mod_poly)) <= 1023). {
+            (*Need to prove bounds differently bc it is not smaller than mod_poly*)
              pose proof (poly_to_int_bounded (x *~ (monomial (Z.to_nat (i - 1)) %~ mod_poly))).
-             split; try rep_lia. rewrite poly_mult_deg in H4. 2: intro Hz; inversion Hz.
+             split; try rep_lia. rewrite poly_mult_deg in H4. 2: solve_poly_zero.
              rewrite deg_x in H4. 
              assert (2 ^ (1 + deg (monomial (Z.to_nat (i - 1)) %~ mod_poly) + 1) - 1 <=
               2 ^ (1 + 8 + 1) - 1). { rewrite <- Z.sub_le_mono_r.
               apply Z.pow_le_mono_r. lia. apply Zplus_le_compat_r. apply Zplus_le_compat_l.
-              pose proof (pmod_lt_deg mod_poly Hpos (monomial (Z.to_nat (i - 1)))). lia. } rep_lia.
-             intro Hmon. pose proof (modulus_poly_monomial (Z.to_nat (i - 1))).
-             rewrite <- poly_to_int_zero_iff in Hmon. lia. }
-           forward_if;
-           replace (force_val (sem_binary_operation' Oshl tuchar tint (Znth (i - 1)
-                     (power_to_index_contents i ++  map Vint (map Int.repr (list_repeat (Z.to_nat (fec_n - i)) 0%Z))))
-                  (Vint (Int.repr 1)))) with 
-           (Vint (Int.repr (poly_to_int (x *~ (monomial (Z.to_nat (i - 1)) %~ mod_poly))))) by apply Hxpoly.
-          ++  (*ugh this is awful, but cant rewrite the Znth beforehand for some reason*)
-             rewrite Znth_app1 in H4. 2: rewrite power_to_index_contents_length; lia.
-             rewrite power_to_index_contents_Znth in H4; try lia. unfold sem_cast_pointer in H4. unfold force_val in H4. 
+              pose proof (pmod_lt_deg mod_poly (monomial (Z.to_nat (i - 1)))). pose proof modulus_poly_deg_bounds; lia. }
+            rep_lia. solve_poly_zero. }
+          forward_if.
+          ++  (*need to simplify condition in H4, not sure why it is not automated*)
+             rewrite power_to_index_contents_Znth in H4 by lia. unfold sem_cast_pointer in H4. unfold force_val in H4. 
              unfold both_int in H4. simpl sem_shift_ii in H4. unfold sem_cast_pointer in H4. rewrite Hshl in H4.
              unfold Int.lt in H4.
              destruct (zlt
@@ -256,275 +167,226 @@ pose proof modulus_pos as Hmodulus.
                  (Int.signed (Int.repr 256))) as [Hif | Hif]. inversion H4. clear H4.
              rewrite !Int.signed_repr in Hif; try rep_lia.
              forward.
-             ** entailer!. rewrite fec_n_eq; lia.
-             ** entailer!. unfold Int.xor. rewrite !unsigned_repr; try rep_lia.
+             ** entailer!.
+             ** rewrite !power_to_index_contents_Znth by lia. entailer!. simpl. 
                  (*Core of proof: this actually finds x^i % f in this case (complicated because x * (x^(i-1) %f) overflows)*)
-                 assert (Hpi : Vint (Int.zero_ext 8 (Int.repr (Z.lxor 
-                  (poly_to_int (x *~ (monomial (Z.to_nat (i - 1)) %~ mod_poly))) modulus))) = 
-                  Vint (Int.repr (poly_to_int (monomial (Z.to_nat i) %~ mod_poly)))). { f_equal.
-                 assert (Hxor : Z.lxor (poly_to_int (x *~ (monomial (Z.to_nat (i - 1)) %~ mod_poly))) modulus =
-                    poly_to_int (monomial (Z.to_nat i) %~ mod_poly)). {
-                  rewrite <- poly_of_int_to_int. rewrite xor_addition; try rep_lia.
-                  assert (Hdeg: deg (x *~ (monomial (Z.to_nat (i - 1)) %~ mod_poly)) = deg mod_poly). {
+                assert (Hdeg: deg (x *~ (monomial (Z.to_nat (i - 1)) %~ mod_poly)) = deg mod_poly). {
                   assert (Hupper: deg mod_poly <= deg (x *~ (monomial (Z.to_nat (i - 1)) %~ mod_poly))). {
-                  rewrite Hdeglog. rewrite <- (poly_of_int_inv (x *~ (monomial (Z.to_nat (i - 1)) %~ mod_poly) )).
-                  rewrite poly_of_int_deg. apply Z.log2_le_mono. rewrite fec_n_eq; lia. apply poly_to_int_pos.
-                  intro Hzero. rewrite poly_mult_zero_iff in Hzero. destruct Hzero. inversion H14.
-                  rewrite <- poly_to_int_zero_iff in H14. 
-                  pose proof (modulus_poly_monomial (Z.to_nat (i-1))). lia. }
+                  rewrite modulus_poly_deg. 
+                  rewrite <- (poly_of_int_inv (x *~ (monomial (Z.to_nat (i - 1)) %~ mod_poly) )).
+                  rewrite poly_of_int_deg. apply Z.log2_le_mono. rep_lia.  apply poly_to_int_pos. solve_poly_zero. }
                   assert (Hlower: deg (monomial (Z.to_nat (i - 1)) %~ mod_poly) < deg mod_poly). {
                   apply pmod_lt_deg. auto. }
-                  assert (Hnonz: monomial (Z.to_nat (i - 1)) %~ mod_poly <> zero). intro Hz.
-                  pose proof (modulus_poly_monomial (Z.to_nat (i-1))). rewrite <- poly_to_int_zero_iff in Hz. lia.
+                  assert (Hnonz: monomial (Z.to_nat (i - 1)) %~ mod_poly <> zero) by solve_poly_zero.
+                  assert (Hx: x <> zero) by solve_poly_zero. 
                   rewrite poly_mult_deg; auto. rewrite poly_mult_deg in Hupper; auto. 
-                  rewrite deg_x. rewrite deg_x in Hupper. lia. all: intro Z; inversion Z. }
+                  rewrite deg_x. rewrite deg_x in Hupper. lia. }
+                assert (Hxor : Z.lxor (poly_to_int (x *~ (monomial (Z.to_nat (i - 1)) %~ mod_poly))) modulus =
+                  poly_to_int (monomial (Z.to_nat i) %~ mod_poly)). {
+                  rewrite <- poly_of_int_to_int. rewrite xor_addition; try rep_lia.
                   rewrite poly_of_int_inv.
                   assert (Hdeglt: deg (x *~ (monomial (Z.to_nat (i - 1)) %~ mod_poly) +~ poly_of_int modulus) < deg mod_poly). {
-                   rewrite poly_add_comm. rewrite <- mod_poly_eq. apply poly_add_deg_same; auto. }
-                  rewrite <- (pmod_refl _ Hpos _ Hdeglt). rewrite <- mod_poly_eq. rewrite pmod_add_distr; auto.
-                  rewrite pmod_same; auto. rewrite poly_add_0_r. rewrite <- (pmod_refl _ Hpos x).
-                  rewrite <- pmod_mult_distr; auto. rewrite <- monomial_expand. rewrite pmod_twice; auto.
-                  f_equal. f_equal. lia. rewrite deg_x. lia. 
-                  rewrite Z.lxor_nonneg. pose proof modulus_pos. rep_lia. }
-                 unfold Int.zero_ext. f_equal. rewrite Zbits.Zzero_ext_mod; try lia.
-                 assert (Hpbound: 0 <= Z.lxor (poly_to_int (x *~ (monomial (Z.to_nat (i - 1)) %~ mod_poly))) modulus < fec_n). {
-                  rewrite Hxor. apply modulus_poly_bound. apply pmod_lt_deg. auto. }
-                 rewrite Zmod_small. 2: { replace (two_p 8) with 256 by reflexivity.
-                 rewrite unsigned_repr; try rep_lia. }
-                 rewrite unsigned_repr; rewrite Hxor. reflexivity. rep_lia. } rewrite Hpi.
-                 rewrite upd_Znth_app2. 2: list_solve.
-                 replace ((i - Zlength (power_to_index_contents i))) with 0%Z by list_solve.
-                 assert (Hlr: (list_repeat (Z.to_nat (fec_n - i)) 0%Z) = 0%Z :: 
+                   rewrite poly_add_comm. rewrite <- mod_poly_eq. apply poly_add_deg_same; auto. solve_poly_zero.  }
+                  rewrite <- (pmod_refl mod_poly _ Hdeglt). rewrite <- mod_poly_eq. rewrite pmod_add_distr; auto.
+                  rewrite pmod_same by auto. rewrite poly_add_0_r. rewrite <- (pmod_refl mod_poly x).
+                  rewrite <- pmod_mult_distr by auto. rewrite <- monomial_expand. rewrite pmod_twice; auto.
+                  f_equal. f_equal. lia. rewrite deg_x. pose proof (modulus_poly_deg_bounds); lia.
+                  rewrite Z.lxor_nonneg. solve_poly_bounds. }
+                unfold Int.xor. rewrite Hshl. rewrite !unsigned_repr by rep_lia. rewrite Hxor. simpl_repr.
+                rewrite upd_Znth_app2 by list_solve. 
+                replace ((i - Zlength (power_to_index_contents i))) with 0%Z by list_solve.
+                assert (Hlr: (list_repeat (Z.to_nat (fec_n - i)) 0%Z) = 0%Z :: 
                     (list_repeat (Z.to_nat fec_n - Z.to_nat (i + 1)) 0%Z)). { 
-                  assert (i < fec_n) by (rewrite fec_n_eq; lia).
-                  replace (Z.to_nat (fec_n - i)) with 
-                    (1%nat + (Z.to_nat fec_n - Z.to_nat (i + 1)))%nat by lia. rewrite <- list_repeat_app.
-                  auto. } rewrite Hlr. simpl. rewrite upd_Znth0. rewrite power_to_index_contents_plus_1; try lia.
-                  rewrite <- app_assoc; simpl. cancel.
+                 replace (Z.to_nat (fec_n - i)) with 
+                 (1%nat + (Z.to_nat fec_n - Z.to_nat (i + 1)))%nat by rep_lia. rewrite <- list_repeat_app. auto. }
+                rewrite Hlr. simpl. rewrite upd_Znth0. rewrite power_to_index_contents_plus_1 by lia.
+                rewrite <- app_assoc; simpl. cancel.
           ++ (*Now on other case of if statement, again need a lot of work to simplify if condition*)
-             rewrite Znth_app1 in H4. 2: rewrite power_to_index_contents_length; lia.
-             rewrite power_to_index_contents_Znth in H4; try lia. unfold sem_cast_pointer in H4. unfold force_val in H4. 
+             rewrite power_to_index_contents_Znth in H4 by lia. unfold sem_cast_pointer in H4. unfold force_val in H4. 
              unfold both_int in H4. simpl sem_shift_ii in H4. unfold sem_cast_pointer in H4. rewrite Hshl in H4.
              unfold Int.lt in H4.  destruct (zlt
              (Int.signed (Int.repr (poly_to_int (x *~ (monomial (Z.to_nat (i - 1)) %~ mod_poly)))))
-             (Int.signed (Int.repr 256))) as [Hlt | ]. inversion H4. clear H4.
-             rewrite !Int.signed_repr in Hlt; try rep_lia.
-             ** forward.
-                --- entailer!. rewrite fec_n_eq; lia.
-                --- entailer!. assert (Hmon : (Vint (Int.zero_ext 8 (Int.repr (poly_to_int
-                     (x *~ (monomial (Z.to_nat (i - 1)) %~ mod_poly)))))) = 
-                      Vint (Int.repr (poly_to_int (monomial (Z.to_nat i) %~ mod_poly)))). {
-                     f_equal. unfold Int.zero_ext. f_equal. rewrite Zbits.Zzero_ext_mod; try lia.
-                     pose proof (poly_to_int_bounded (x *~ (monomial (Z.to_nat (i - 1)) %~ mod_poly))) as Hlb.
-                     replace (two_p 8) with (256) by reflexivity.
-                     rewrite Zmod_small; try rep_lia. all: rewrite unsigned_repr; try rep_lia. f_equal.
-                     assert (Hdeg: deg (x *~ (monomial (Z.to_nat (i - 1)) %~ mod_poly)) < deg mod_poly). {
-                     rewrite Hdeglog. rewrite <- (poly_of_int_inv (x *~ (monomial (Z.to_nat (i - 1)) %~ mod_poly))).
-                     replace (Z.log2 fec_n) with 8 by (rewrite fec_n_eq; reflexivity).
-                     rewrite poly_of_int_deg. 
-                     assert (Hle: poly_to_int (x *~ (monomial (Z.to_nat (i - 1)) %~ mod_poly)) <= 255) by lia.
-                     apply Z.log2_le_mono in Hle. replace (Z.log2 255) with 7 in Hle by reflexivity. lia.
-                     apply poly_to_int_pos. intro Hz. rewrite poly_mult_zero_iff in Hz. destruct Hz.
-                     inversion H14. rewrite <- poly_to_int_zero_iff in H14. 
-                     pose proof (modulus_poly_monomial (Z.to_nat (i-1))). lia. }
-                     rewrite <- (pmod_refl _ Hpos _ Hdeg). rewrite <- (pmod_refl _ Hpos x).
-                     rewrite <- pmod_mult_distr; auto. rewrite <- monomial_expand. f_equal. f_equal. lia.
-                     rewrite deg_x. lia. }
-                     rewrite Hmon.  rewrite upd_Znth_app2. 2: list_solve.
-                     replace ((i - Zlength (power_to_index_contents i))) with 0%Z by list_solve.
-                     assert (Hlr: (list_repeat (Z.to_nat (fec_n - i)) 0%Z) = 0%Z :: 
-                      (list_repeat (Z.to_nat fec_n - Z.to_nat (i + 1)) 0%Z)). { 
-                      assert (i < fec_n) by (rewrite fec_n_eq; lia).
-                      replace (Z.to_nat (fec_n - i)) with 
-                      (1%nat + (Z.to_nat fec_n - Z.to_nat (i + 1)))%nat by lia. rewrite <- list_repeat_app.
-                      auto. } rewrite Hlr. simpl. rewrite upd_Znth0. rewrite power_to_index_contents_plus_1; try lia.
-                     rewrite <- app_assoc; simpl. cancel.
-             ** inversion H4.
-      * (*Now need to prove [fec_2_power] part*)
-        assert (Hbound: 0 <= poly_to_int (monomial (Z.to_nat i) %~ mod_poly) < fec_n). { apply modulus_poly_bound.
-        apply pmod_lt_deg; auto. } rewrite fec_n_eq in Hbound.
+             (Int.signed (Int.repr 256))) as [Hlt | ]. 2: inversion H4. clear H4.
+             rewrite !Int.signed_repr in Hlt by rep_lia. forward.
+             --- entailer!.
+             --- entailer!. rewrite !power_to_index_contents_Znth by lia. simpl. rewrite Hshl. simpl_repr.
+                 assert (Hdeg: deg (x *~ (monomial (Z.to_nat (i - 1)) %~ mod_poly)) < deg mod_poly). {
+                   rewrite modulus_poly_deg. rewrite <- (poly_of_int_inv (x *~ (monomial (Z.to_nat (i - 1)) %~ mod_poly))).
+                   replace (Z.log2 fec_n) with 8 by (rewrite fec_n_eq; reflexivity).
+                   rewrite poly_of_int_deg. 
+                   assert (Hle: poly_to_int (x *~ (monomial (Z.to_nat (i - 1)) %~ mod_poly)) <= 255) by lia.
+                   apply Z.log2_le_mono in Hle. replace (Z.log2 255) with 7 in Hle by reflexivity. lia.
+                   apply poly_to_int_pos. solve_poly_zero. }
+                 assert (Hmon: (x *~ (monomial (Z.to_nat (i - 1)) %~ mod_poly)) = monomial (Z.to_nat i) %~ mod_poly). {
+                   rewrite <- (pmod_refl mod_poly _ Hdeg).
+                   rewrite pmod_mult_distr; auto. rewrite pmod_twice by auto. rewrite <- pmod_mult_distr by auto.
+                   rewrite <- monomial_expand. f_equal. f_equal. lia. } rewrite Hmon.
+                 rewrite upd_Znth_app2 by list_solve.
+                 replace ((i - Zlength (power_to_index_contents i))) with 0%Z by list_solve.
+                 assert (Hlr: (list_repeat (Z.to_nat (fec_n - i)) 0%Z) = 0%Z :: 
+                  (list_repeat (Z.to_nat fec_n - Z.to_nat (i + 1)) 0%Z)). { 
+                  assert (i < fec_n) by (rewrite fec_n_eq; lia).
+                  replace (Z.to_nat (fec_n - i)) with 
+                  (1%nat + (Z.to_nat fec_n - Z.to_nat (i + 1)))%nat by lia. rewrite <- list_repeat_app.
+                  auto. } rewrite Hlr. simpl. rewrite upd_Znth0. rewrite power_to_index_contents_plus_1; try lia.
+                 rewrite <- app_assoc; simpl. cancel.
+      * (*Now need to prove [fec_2_power] part*) 
+        assert (Hbound: 0 <= poly_to_int (monomial (Z.to_nat i) %~ mod_poly) < fec_n) by solve_poly_bounds. 
         forward.
-        -- entailer!. rewrite fec_n_eq; lia.
-        -- entailer!. rewrite Znth_app1. 2: solve_prop_length. rewrite power_to_index_contents_Znth; try lia. simpl.
-           rewrite unsigned_repr; rep_lia.
-        -- rewrite Znth_app1. 2: solve_prop_length. rewrite power_to_index_contents_Znth; try lia.
-           forward.
-           ++ entailer!. rewrite fec_n_eq; lia.
-           ++ forward. entailer!.
-              (*now continue and show loop invariant preserved - this is a bit tricky because
-              we are not filling up the array in an orderly way - need to show that we dont fill in the same
-              spot twice (other than 0, special case). We rely on the uniqueness of [find_power] *)
-              Exists (i+1). Exists ((upd_Znth (poly_to_int (monomial (Z.to_nat i) %~ mod_poly)) l i)).
-              (*Now, let's prove the invariant is preserved*) 
-              pose proof field_size_fec_n as S1. rewrite fec_n_eq in H8. entailer!.  
-              (*rewrite Zlength_upd_Znth in H9. rewrite? Zlength_map in H9. split.*)
-                ** split; intros.
-                  --- assert (Hfp: 0 < find_power mod_poly (poly_of_int z) < i \/ 
-                      find_power mod_poly (poly_of_int z) = i) by lia. destruct Hfp as [Hfp | Hfp].
-                    +++ (*if smaller than i - MUST be different than the current one - uniqueness*)
-                        rewrite upd_Znth_diff. apply H0. all: try lia. list_solve. list_solve.
-                        intro Hz. assert (find_power mod_poly (poly_of_int z) = i).
-                        symmetry. rewrite <- find_power_iff.
-                        split. rewrite Hz. rewrite poly_of_int_inv. reflexivity. rewrite S1.
-                        rewrite fec_n_eq; lia. all: auto.
-                        intro Hzero. apply poly_of_int_zero in Hzero. lia.
-                        apply polys_deg_bounded. lia. lia.
-                    +++ assert (Hz: z = (poly_to_int (monomial (Z.to_nat i) %~ mod_poly))). { symmetry in Hfp.
-                        rewrite <- find_power_iff in Hfp. destruct Hfp as [Hfp  Hi]. rewrite <- poly_of_int_to_int.
-                        symmetry. assumption. lia. all: auto. intro Hzero. rewrite poly_of_int_zero in Hzero. lia.
-                        apply polys_deg_bounded. lia. } 
-                        rewrite Hz. rewrite upd_Znth_same. rewrite <- Hz. rewrite <- Hfp. reflexivity.
-                        list_solve.
-                  --- rewrite upd_Znth_diff. assumption. list_solve. list_solve. 
-                      pose proof (modulus_poly_monomial (Z.to_nat i)). lia.
-                ** rewrite upd_Znth_map.  assert (Hl: (map Vint
-                    (upd_Znth (poly_to_int (monomial (Z.to_nat i) %~ mod_poly)) 
-                    (map Int.repr l) (Int.zero_ext 8 (Int.repr i)))) =  (map Vint
-                    (map Int.repr (upd_Znth (poly_to_int (monomial (Z.to_nat i) %~ mod_poly)) l i)))). {
-                    f_equal. rewrite <- upd_Znth_map. f_equal. unfold Int.zero_ext.
-                    f_equal. rewrite Zbits.Zzero_ext_mod; try lia. replace (two_p 8) with (256) by reflexivity.
-                    rewrite Zmod_small; try rewrite unsigned_repr; try rep_lia. } rewrite Hl. cancel.
-                    replace ((Z.to_nat fec_n - Z.to_nat (i + 1))%nat) with (Z.to_nat (fec_n - (i + 1))) by lia. cancel.
+        -- entailer!. (*rewrite fec_n_eq; lia.*)
+        -- entailer!. rewrite Znth_app1 by solve_prop_length. rewrite power_to_index_contents_Znth by lia. solve_poly_bounds. 
+        -- rewrite Znth_app1 by solve_prop_length. rewrite power_to_index_contents_Znth by lia.
+           forward. forward. 
+          (*now continue and show loop invariant preserved - this is a bit tricky because
+          we are not filling up the array in an orderly way - need to show that we dont fill in the same
+          spot twice (other than 0, special case). We rely on the uniqueness of [find_power] *)
+          Exists (i+1). Exists ((upd_Znth (poly_to_int (monomial (Z.to_nat i) %~ mod_poly)) l i)).
+          (*Now, let's prove the invariant is preserved*) 
+          pose proof field_size_fec_n as S1. entailer!.  
+            ** split; intros.
+              --- assert (Hfp: 0 < find_power mod_poly (poly_of_int z) < i \/ 
+                  find_power mod_poly (poly_of_int z) = i) by lia. destruct Hfp as [Hfp | Hfp].
+                +++ (*if smaller than i - MUST be different than the current one - uniqueness*)
+                    rewrite upd_Znth_diff. apply H0. all: try lia. list_solve. list_solve.
+                    intro Hz. assert (find_power mod_poly (poly_of_int z) = i).
+                    symmetry. rewrite <- find_power_iff.
+                    split. rewrite Hz. rewrite poly_of_int_inv. reflexivity. rep_lia. apply mod_poly_PrimPoly. solve_poly_zero.
+                    solve_poly_bounds. lia.
+                +++ assert (Hz: z = (poly_to_int (monomial (Z.to_nat i) %~ mod_poly))). { symmetry in Hfp.
+                    rewrite <- find_power_iff in Hfp. destruct Hfp as [Hfp  Hi]. rewrite <- poly_of_int_to_int.
+                    symmetry. assumption. lia. apply mod_poly_PrimPoly. solve_poly_zero. solve_poly_bounds.  } 
+                    rewrite Hz. rewrite upd_Znth_same. rewrite <- Hz. rewrite <- Hfp. reflexivity.
+                    list_solve.
+              --- rewrite upd_Znth_diff. assumption. list_solve. list_solve. 
+                  pose proof (modulus_poly_monomial (Z.to_nat i)). lia.
+            ** rewrite upd_Znth_map.  assert (Hl: (map Vint
+                (upd_Znth (poly_to_int (monomial (Z.to_nat i) %~ mod_poly)) 
+                (map Int.repr l) (Int.zero_ext 8 (Int.repr i)))) =  (map Vint
+                (map Int.repr (upd_Znth (poly_to_int (monomial (Z.to_nat i) %~ mod_poly)) l i)))). {
+                f_equal. rewrite <- upd_Znth_map. f_equal. solve_repr_int. } rewrite Hl. cancel.
+                replace ((Z.to_nat fec_n - Z.to_nat (i + 1))%nat) with (Z.to_nat (fec_n - (i + 1))) by lia. cancel.
     + (*end of first loop - need to prove postcondition*) forward. entailer!.
-      assert (i = fec_n). rewrite fec_n_eq; lia. subst. replace (Z.to_nat (fec_n - fec_n)) with 0%nat by lia.
-      simpl. rewrite app_nil_r. cancel. 
+      assert (i = fec_n) by rep_lia. subst. replace (Z.to_nat (fec_n - fec_n)) with 0%nat by lia.
+      simpl. rewrite app_nil_r. unfold INDEX_TABLES. cancel. 
       (*The only nontrivial part: l is the correct index_to_power_contents list*)
       assert (Hl: (map Vint (map Int.repr l)) =
       (map Vint (map Int.repr (prop_list (fun z : Z => find_power mod_poly (poly_of_int z)) fec_n)))). {
         f_equal. f_equal. apply Znth_eq_ext. rewrite prop_list_length. list_solve. lia. intros i Hi.
         rewrite? Zlength_map in H7. rewrite H7 in Hi.
         destruct (Z.eq_dec 0 i).
-        - subst. rewrite H1. rewrite prop_list_Znth. assert (Hzero: poly_of_int 0 = zero) by 
-          (rewrite poly_of_int_zero; lia). rewrite Hzero. rewrite find_power_zero. reflexivity. all: assumption. 
-        - rewrite H0; try lia. rewrite prop_list_Znth. reflexivity. assumption. 
-          pose proof (find_power_spec mod_poly Hpos Hprim Hnotx (poly_of_int i)) as Hfp.
-          assert (Hnz: poly_of_int i <> zero). intro Hz. rewrite poly_of_int_zero in Hz. lia.
-          specialize (Hfp Hnz (polys_deg_bounded _ Hi)). destruct Hfp as [ ? Hfpbound].
-          rewrite field_size_fec_n in Hfpbound. lia. } rewrite Hl. unfold index_to_power_contents. cancel.
+        - subst. rewrite H1. rewrite prop_list_Znth. rewrite_zero. rewrite (@find_power_zero _ mod_poly_PosPoly). reflexivity.
+          apply mod_poly_PrimPoly. auto. 
+        - pose_power (poly_of_int i) Hfp Hfpbound. rewrite H0; try lia. rewrite prop_list_Znth by rep_lia.
+          reflexivity. }
+        rewrite Hl. unfold index_to_power_contents. cancel.
   - (*Second loop: calculate inverses*) 
-    pose proof field_size_fec_n as Hfieldsize.
+    pose proof field_size_fec_n as Hfieldsize. 
+    assert (Hmodpos: deg mod_poly > 0) by (pose proof modulus_poly_deg_bounds; rep_lia).
+    assert (Hirred: irreducible mod_poly) by (apply (@f_irred _ _ mod_poly_PrimPoly)).
+    assert (Hmodnotx : mod_poly <> x) by (apply (@Hnotx _ _ mod_poly_PrimPoly)).
+    clear Hpospoly.
     forward_for_simple_bound 256%Z (EX (i : Z) (l: list Z),
-    PROP (0 <= i <= fec_n  /\ Znth 0 l = 0%Z /\ (forall z, 0 < z < fec_n -> 0 <= poly_to_int (poly_inv mod_poly modulus_poly_deg_pos (poly_of_int z)) < i ->
-          Znth z l = poly_to_int (poly_inv mod_poly modulus_poly_deg_pos (poly_of_int z))
+    PROP (0 <= i <= fec_n  /\ Znth 0 l = 0%Z /\ (forall z, 0 < z < fec_n -> 
+          0 <= poly_to_int (poly_inv mod_poly (poly_of_int z)) < i ->
+          Znth z l = poly_to_int (poly_inv mod_poly (poly_of_int z))
       ))
     LOCAL (temp _mod (Vint (Int.repr modulus));  gvars gv)
-    SEP (data_at Ews (tarray tuchar fec_n) (power_to_index_contents fec_n) (gv _fec_2_index);
-        data_at Ews (tarray tuchar fec_n) index_to_power_contents (gv _fec_2_power);
-        data_at Ews (tarray tuchar fec_n) (map Vint (map Int.repr l)) (gv _fec_invefec ))).
-    + Exists (list_repeat (Z.to_nat fec_n ) 0%Z). entailer!. rewrite Znth_list_repeat_inrange.
-      reflexivity. lia.
+    SEP (INDEX_TABLES gv;
+         data_at Ews (tarray tuchar fec_n) (map Vint (map Int.repr l)) (gv _fec_invefec ))).
+    + Exists (list_repeat (Z.to_nat fec_n ) 0%Z). entailer!. rewrite Znth_list_repeat_inrange; rep_lia.
     + assert (Hfpbound: 0 <= find_power mod_poly (poly_of_int i) <= fec_n - 1). {
        destruct (Z.eq_dec i 0).
-       - subst. assert (Hz: (poly_of_int 0 = zero)) by (rewrite poly_of_int_zero; lia). rewrite Hz.
-         rewrite find_power_zero. lia. all: assumption.
-       - pose proof (find_power_spec _ Hpos Hprim Hnotx (poly_of_int i)) as Hfp.
-         assert (poly_of_int i <> zero). intro Hz. rewrite poly_of_int_zero in Hz. lia.
-         assert (deg (poly_of_int i) < deg mod_poly). apply polys_deg_bounded. rewrite fec_n_eq; lia. 
-         specialize (Hfp H0 H1). rewrite fec_n_eq; destruct Hfp; rep_lia. }
+       - subst. rewrite_zero.  rewrite (@find_power_zero _ _ mod_poly_PrimPoly). lia.
+       - solve_poly_bounds. } unfold INDEX_TABLES; Intros. 
       forward.
-      * entailer!. rewrite fec_n_eq; lia.
-      * entailer!. rewrite index_to_power_contents_Znth. 2: rewrite fec_n_eq; lia. simpl.
-        rewrite unsigned_repr; rep_lia.
-      * rewrite index_to_power_contents_Znth. 2: rewrite fec_n_eq; lia.
+      * entailer!.
+      * entailer!. rewrite index_to_power_contents_Znth by rep_lia. solve_poly_bounds. 
+      * rewrite index_to_power_contents_Znth by rep_lia. 
         assert (Hinvbound: 0 <=
             poly_to_int (monomial (Z.to_nat (255 - find_power mod_poly (poly_of_int i))) %~ mod_poly) <
-            256). { rewrite <- fec_n_eq. apply modulus_poly_bound. apply pmod_lt_deg. auto. }
+            256) by solve_poly_bounds. 
         forward.
-        -- entailer!. rewrite fec_n_eq; lia.
-        -- entailer!. rewrite power_to_index_contents_Znth. simpl.
-           rewrite unsigned_repr; rep_lia. rewrite fec_n_eq; lia.
-        -- rewrite power_to_index_contents_Znth. 2: { simpl. rewrite fec_n_eq; lia. }
+        -- entailer!.
+        -- entailer!. rewrite power_to_index_contents_Znth; solve_poly_bounds. 
+        -- rewrite power_to_index_contents_Znth by solve_poly_bounds.
            forward.
-          ++ entailer!. rewrite fec_n_eq; lia.
+          ++ entailer!.
           ++ (*loop invariant preservation*)
               Exists (upd_Znth (poly_to_int (monomial (Z.to_nat 
                 (fec_n - 1 - find_power mod_poly (poly_of_int i))) %~ mod_poly)) l i).
             entailer!.
-            ** assert (Hlen: Zlength l = fec_n) by list_solve. split. rewrite fec_n_eq; lia. split.
+            ** assert (Hlen: Zlength l = fec_n) by list_solve. split.
               --- (*handle 0 case separately*)
                   destruct (Z.eq_dec 0%Z (poly_to_int (monomial (Z.to_nat 
                     (fec_n - 1 - find_power mod_poly (poly_of_int i))) %~ mod_poly))).
-                +++ rewrite <- poly_of_int_to_int in e. assert (Hz: poly_of_int 0 = zero) by (rewrite poly_of_int_zero; lia).
-                    rewrite Hz in e. exfalso. 
+                +++ rewrite <- poly_of_int_to_int in e. rewrite_zero. exfalso. 
                     apply (irred_doesnt_divide_monomial mod_poly (Z.to_nat (fec_n - 1 - find_power mod_poly (poly_of_int i)))).
-                    all: try assumption. rewrite divides_pmod_iff. unfold divides_pmod. apply e. left. 
-                    assumption. lia.
-                +++ rewrite upd_Znth_diff. assumption. list_solve. rewrite Hlen; rewrite fec_n_eq; auto. 
-                    assumption.
-              --- intros z Hzf Hpi1. 
-                  assert (0 <=  poly_to_int (poly_inv mod_poly modulus_poly_deg_pos (poly_of_int z)) < i \/
-                    poly_to_int (poly_inv mod_poly modulus_poly_deg_pos (poly_of_int z)) = i) by lia. 
-                  destruct H14 as [Hilt | Hi].
-                +++ rewrite upd_Znth_diff. apply H2; try assumption; try lia. list_solve.
-                    rewrite Hlen; rewrite fec_n_eq; auto. (*contradiction: i and z are inverses*)
-                    intro Hz. assert (poly_to_int (poly_inv mod_poly modulus_poly_deg_pos (poly_of_int z)) = i). {
-                    symmetry. rewrite <- poly_of_int_to_int. 2 : lia. 
-                    destruct (Z.eq_dec z 0%Z).
-                    - subst. symmetry in e. rewrite <- poly_of_int_to_int in e; try lia.
-                      assert (Hzero: poly_of_int 0 = zero) by (rewrite poly_of_int_zero; lia). rewrite Hzero in e.
-                      exfalso. apply (irred_doesnt_divide_monomial mod_poly 
-                        (Z.to_nat (fec_n - 1 - find_power mod_poly (poly_of_int i)))); try assumption.
-                      rewrite divides_pmod_iff. unfold divides_pmod. assumption. left. assumption.
-                    - symmetry. rewrite <- poly_inv_iff. rewrite Hz. rewrite poly_of_int_inv.
-                      pose proof (find_power_spec _ Hpos Hprim Hnotx (poly_of_int i)) as Hfp.
-                      assert (Hinz: poly_of_int i <> zero). { intro Hzero. rewrite poly_of_int_zero in Hzero. lia. }
-                      assert (Hdegi: deg (poly_of_int i) < deg mod_poly). apply polys_deg_bounded; rewrite fec_n_eq; lia.
-                      specialize (Hfp Hinz Hdegi). destruct Hfp as [Hi Hfp_bound]. rewrite Hi at 2. split. 2: assumption.
-                      rewrite pmod_mult_reduce. rewrite poly_mult_comm. rewrite pmod_mult_reduce. rewrite monomial_exp_law.
-                      replace ((Z.to_nat (find_power mod_poly (poly_of_int i)) +
-                      Z.to_nat (fec_n - 1 - find_power mod_poly (poly_of_int i)))%nat) with (Z.to_nat (fec_n - 1)) by lia.
-                      replace (Z.to_nat (fec_n - 1)) with (0%nat + Z.to_nat (fec_n -1))%nat by lia.
-                      rewrite <- Hfieldsize. replace (Z.to_nat (Z.of_nat (field_size mod_poly))) with
-                      (field_size mod_poly) by lia.
-                      rewrite <- monomial_add_field_size. rewrite monomial_0. apply pmod_refl.
-                      all: try assumption. assert (0%Z = deg one) by (rewrite deg_one; reflexivity). lia.
-                      intro Hzero. rewrite pmod_refl in Hzero. rewrite poly_of_int_zero in Hzero. lia.
-                      assumption. apply polys_deg_bounded. lia. } lia.
-                +++ (*proving the actual update, since i and z are correctly inverses this time*)
-                    symmetry in Hi. rewrite <- poly_of_int_to_int in Hi. 2: lia.
-                    assert (Hzi : poly_of_int z = poly_inv mod_poly modulus_poly_deg_pos (poly_of_int i)). {
-                      rewrite poly_inv_sym. rewrite Hi. reflexivity. all: try assumption. apply polys_deg_bounded.
-                      rewrite fec_n_eq; lia. apply polys_deg_bounded. lia. }
-                    assert (Hz: z = (poly_to_int (monomial (Z.to_nat (fec_n - 1 - find_power mod_poly (poly_of_int i))) %~ mod_poly))). {
-                      rewrite <- poly_of_int_to_int. rewrite Hzi. 2: lia.
-                      destruct (destruct_poly (poly_of_int i)).
-                      - rewrite e in Hi. rewrite <- poly_inv_zero in Hi. rewrite pmod_refl in Hi. 
-                        rewrite poly_of_int_zero in Hi. lia. all: try assumption. apply polys_deg_bounded.
-                        lia.
-                      - rewrite <- poly_inv_iff. split. pose proof (find_power_spec _ Hpos Hprim Hnotx (poly_of_int i) n) as Hfp.
-                        assert (Hideg: deg (poly_of_int i) < deg mod_poly). { apply polys_deg_bounded; rewrite fec_n_eq; lia. }
-                        specialize (Hfp Hideg). destruct Hfp as [Hpi Hfp_bound]. rewrite Hpi at 1. rewrite pmod_mult_reduce.
-                        rewrite poly_mult_comm. rewrite pmod_mult_reduce. rewrite monomial_exp_law.
-                        replace ((Z.to_nat (fec_n - 1 - find_power mod_poly (poly_of_int i)) +
-                          Z.to_nat (find_power mod_poly (poly_of_int i))))%nat with (0 + Z.to_nat (fec_n - 1))%nat by lia.
-                        rewrite <- Hfieldsize. replace ( Z.to_nat (Z.of_nat (field_size mod_poly))) with (field_size mod_poly)
-                        by lia. rewrite <- monomial_add_field_size. rewrite monomial_0. apply pmod_refl.
-                        all: try assumption. assert (0%Z = deg one) by (rewrite deg_one; reflexivity). lia.
-                        apply pmod_lt_deg; assumption. rewrite pmod_refl; try assumption. 
-                        apply polys_deg_bounded; rewrite fec_n_eq; lia. }
-                    rewrite <- Hz. rewrite upd_Znth_same. rewrite <- poly_of_int_to_int. assumption.
-                    lia. list_solve.
+                    apply Hpos. apply (@f_irred _ _ mod_poly_PrimPoly). apply (@Hnotx _ _ mod_poly_PrimPoly).
+                    rewrite divides_pmod_iff. unfold divides_pmod. apply e. left. solve_poly_zero. lia. 
+                +++ rewrite upd_Znth_diff. assumption. list_solve. rewrite Hlen. solve_poly_bounds. apply n. 
+        --- intros z Hzf Hpi1. 
+            (*Will come in handy for both branches*)
+            assert (Hpowmod: monomial (Z.to_nat (find_power mod_poly (poly_of_int i)) +
+              Z.to_nat (fec_n - 1 - find_power mod_poly (poly_of_int i))) %~ mod_poly = one). {
+              replace ((Z.to_nat (find_power mod_poly (poly_of_int i)) +
+               Z.to_nat (fec_n - 1 - find_power mod_poly (poly_of_int i)))%nat) with (Z.to_nat (fec_n - 1)) by lia.
+              rewrite (@monomial_powers_eq_mod _ _ mod_poly_PrimPoly _ 0). rewrite monomial_0. apply pmod_refl; auto.
+              apply mod_poly_PosPoly. apply (@deg_gt_one _ _ mod_poly_PrimPoly). apply Nat2Z.inj. rewrite mod_Zmod by rep_lia.
+              rewrite mod_Zmod by rep_lia. rewrite Hfieldsize. rewrite Z2Nat.id by lia. rewrite Z_mod_same_full.
+              rewrite Z.mod_0_l; lia. }
+              assert (0 <=  poly_to_int (poly_inv mod_poly (poly_of_int z)) < i \/
+                poly_to_int (poly_inv mod_poly (poly_of_int z)) = i) by lia. 
+              destruct H14 as [Hilt | Hi].
+            +++ rewrite upd_Znth_diff. apply H2; try assumption; try lia. list_solve. rewrite Hlen. solve_poly_bounds. 
+                (*contradiction: i and z are inverses*)
+                intro Hz. assert (poly_to_int (poly_inv mod_poly (poly_of_int z)) = i). {
+                symmetry. rewrite <- poly_of_int_to_int by lia. 
+                destruct (Z.eq_dec z 0%Z).
+                - subst. symmetry in e. rewrite <- poly_of_int_to_int in e; try lia. rewrite_zero.
+                  exfalso. apply (irred_doesnt_divide_monomial mod_poly 
+                    (Z.to_nat (fec_n - 1 - find_power mod_poly (poly_of_int i)))); try assumption.
+                  rewrite divides_pmod_iff. unfold divides_pmod. assumption. left. solve_poly_zero.
+                - symmetry. rewrite <- poly_inv_iff; [| assumption | ]. rewrite Hz.
+                  rewrite poly_of_int_inv. pose_power (poly_of_int i) Hi Hfp_bound. rewrite Hi at 2. split. 
+                  2: solve_poly_bounds. pose proof mod_poly_PosPoly as HmodPos.
+                  rewrite pmod_mult_reduce by auto. rewrite poly_mult_comm. rewrite pmod_mult_reduce by auto. 
+                  rewrite monomial_exp_law. assumption. rewrite pmod_refl; auto. solve_poly_zero. apply mod_poly_PosPoly.
+                  solve_poly_bounds. } lia. 
+            +++ (*proving the actual update, since i and z are correctly inverses this time*)
+                symmetry in Hi. rewrite <- poly_of_int_to_int in Hi by lia.
+                assert (Hzi : poly_of_int z = poly_inv mod_poly (poly_of_int i)). {
+                  rewrite poly_inv_sym; auto; solve_poly_bounds.  }
+                assert (Hz: z = (poly_to_int (monomial (Z.to_nat (fec_n - 1 - find_power mod_poly (poly_of_int i))) %~ mod_poly))). {
+                  rewrite <- poly_of_int_to_int. rewrite Hzi by lia.
+                  destruct (destruct_poly (poly_of_int i)).
+                  - rewrite e in Hi. rewrite <- poly_inv_zero in Hi by auto. rewrite pmod_refl in Hi; try auto. 
+                    rewrite poly_of_int_zero in Hi. lia. apply mod_poly_PosPoly. solve_poly_bounds. 
+                  - rewrite <- poly_inv_iff; auto. split. pose_power (poly_of_int i) Hpi Hfp_bound.
+                    rewrite Hpi at 1. rewrite pmod_mult_reduce by apply mod_poly_PosPoly.
+                    rewrite poly_mult_comm. rewrite pmod_mult_reduce by apply mod_poly_PosPoly. rewrite monomial_exp_law.
+                    rewrite Nat.add_comm. apply Hpowmod. apply pmod_lt_deg; auto. apply mod_poly_PosPoly. rewrite pmod_refl; auto.
+                    apply mod_poly_PosPoly. 
+                    solve_poly_bounds.
+                  - lia. }
+                rewrite <- Hz. rewrite upd_Znth_same. rewrite <- poly_of_int_to_int. assumption.
+                lia. list_solve.
             ** assert (Hl: (upd_Znth
                 (poly_to_int (monomial (Z.to_nat (255 - find_power mod_poly (poly_of_int i))) %~ mod_poly))
                 (map Vint (map Int.repr l)) (Vint (Int.zero_ext 8 (Int.repr i)))) = 
                 (map Vint (map Int.repr (upd_Znth (poly_to_int
                   (monomial (Z.to_nat (fec_n - 1 - find_power mod_poly (poly_of_int i))) %~ mod_poly)) l
-                  i)))). { rewrite upd_Znth_map. f_equal. rewrite <- upd_Znth_map. f_equal. unfold Int.zero_ext.
-                rewrite fec_n_eq; simpl. reflexivity. unfold Int.zero_ext. f_equal. rewrite Zbits.Zzero_ext_mod.
-                replace (two_p 8) with (256) by reflexivity.
-                 rewrite Zmod_small. all: try(rewrite unsigned_repr; rep_lia). lia. } 
-               rewrite Hl. cancel.
+                  i)))). { rewrite upd_Znth_map. f_equal. rewrite <- upd_Znth_map. repeat(f_equal). rep_lia.
+                solve_repr_int.  } 
+               rewrite Hl. unfold INDEX_TABLES; cancel.
     + (*postcondition of 2nd loop*)
-      Intros l. entailer!.
+      Intros l. unfold FIELD_TABLES; unfold INDEX_TABLES. entailer!.
       assert (Hl: (map Vint (map Int.repr l)) = (inverse_contents fec_n)). {
         unfold inverse_contents. f_equal. f_equal. apply Znth_eq_ext. rewrite prop_list_length. list_solve. lia.
         intros i Hi.
-        rewrite prop_list_Znth. 2: list_solve. assert (i = 0%Z \/ 0 < i) by lia. destruct H11 as [Hiz | Hipos].
-        - subst. rewrite H0. assert (Hz: poly_of_int 0 = zero) by (rewrite poly_of_int_zero; lia). rewrite Hz.
-          rewrite poly_inv_of_zero. symmetry. rewrite poly_to_int_zero_iff. reflexivity. all: try assumption.
-        - rewrite H1. reflexivity. list_solve. 
-          rewrite <- fec_n_eq. apply modulus_poly_bound.
-          pose proof (poly_inv_spec _ modulus_poly_deg_pos Hirred (poly_of_int i)) as Hinv. apply Hinv.
-          rewrite pmod_refl; auto. intro Hzero. rewrite poly_of_int_zero in Hzero. lia.
-          apply polys_deg_bounded; try rep_lia. list_solve. } rewrite Hl. cancel.
+        rewrite prop_list_Znth by list_solve. assert (i = 0%Z \/ 0 < i) by lia. destruct H11 as [Hiz | Hipos].
+        - subst. rewrite H0. rewrite_zero. rewrite poly_inv_of_zero. symmetry. rewrite poly_to_int_zero_iff.
+          reflexivity. auto.
+        - rewrite H1. reflexivity. list_solve. replace (Zlength l) with fec_n in Hi by list_solve. 
+          pose_inv (poly_of_int i) A B. solve_poly_bounds. }
+        rewrite Hl. cancel.
 Qed.
